Prove 2 admitted lemmas

code/ecdsap256sha2/Hacl.Math.fst
@@ -144,3 +144,46 @@ assume
 val lemma_l_ferm: unit -> Lemma
   (let r = modp_inv2_prime (pow2 256) prime_p256_order in
   (pow r (prime_p256_order - 1) % prime_p256_order == 1))
+
+
+val lemma_multiplication_not_mod_prime_left: a:nat{a < prime256} -> Lemma
+  (requires a * (modp_inv2 (pow2 256)) % prime256 == 0)
+  (ensures a == 0)
+
+let lemma_multiplication_not_mod_prime_left a =
+  let b = modp_inv2 (pow2 256) in
+  lemma_mod_mul_distr_r a b prime256;
+  assert (a * b % prime256 == a * (b % prime256) % prime256);
+  let r = -26959946654596436328278158470660195847911760999080590586820792680449 in
+  let s = 26959946660873538059280334323183841250350249843923952699046031785985 in
+  assert_norm (r * prime256 + s * b == 1);
+  swap_mul a b;
+  assert (b * a % prime256 == 0);
+  euclid prime256 b a r s;
+  assert (a % prime256 == 0);
+  small_mod a prime256
+
+val lemma_multiplication_not_mod_prime: a:nat{a < prime256} ->
+  Lemma (a * (modp_inv2 (pow2 256)) % prime256 == 0 <==> a == 0)
+
+let lemma_multiplication_not_mod_prime a =
+  Classical.move_requires lemma_multiplication_not_mod_prime_left a
+
+
+val lemma_modular_multiplication_p256: a:nat{a < prime256} -> b:nat{b < prime256} -> Lemma
+  (requires a * modp_inv2 (pow2 256) % prime256 == b * modp_inv2 (pow2 256) % prime256)
+  (ensures  a == b)
+
+let lemma_modular_multiplication_p256 a b =
+  let c = modp_inv2 (pow2 256) in
+  mod_sub prime256 (a * c) (b * c);
+  assert (c * (a - b) % prime256 = 0);
+  let r = -26959946654596436328278158470660195847911760999080590586820792680449 in
+  let s = 26959946660873538059280334323183841250350249843923952699046031785985 in
+  assert_norm (r * prime256 + s * c = 1);
+  euclid prime256 c (a - b) r s;
+  assert ((a - b) % prime256 = 0);
+  sub_mod prime256 a b;
+  assert (a % prime256 == b % prime256);
+  FStar.Math.Lemmas.modulo_lemma a prime256;
+  FStar.Math.Lemmas.modulo_lemma b prime256
